Added more design precondition laws

UTP/ITree_Designs.thy
@@ -4,9 +4,11 @@ theory ITree_Designs
   imports ITree_WP
 begin
 
-text \<open> The precondition captures the initial states that do not give the possibility of divergence. \<close>
+named_theorems dpre
 
-definition itree_pre :: "('e, 's) htree \<Rightarrow> ('s \<Rightarrow> bool)" where
+text \<open> The design precondition captures the initial states that do not give the possibility of divergence. \<close>
+
+definition itree_pre :: "('e, 'r, 's) ktree \<Rightarrow> ('r \<Rightarrow> bool)" where
 "itree_pre P = (\<lambda> s. \<not> (\<exists> es. P s \<midarrow>es\<leadsto> diverge))"
 
 lemma itree_pre_div_free: "itree_pre P = (\<lambda> s. div_free (P s))"
@@ -14,29 +16,36 @@ lemma itree_pre_div_free: "itree_pre P = (\<lambda> s. div_free (P s))"
 
 expr_ctr itree_pre
 
-definition refined_by :: "('e, 's) htree \<Rightarrow> ('e, 's) htree \<Rightarrow> bool" (infix "\<sqsubseteq>" 50) where
+definition refined_by :: "('e, 'r, 's) ktree \<Rightarrow> ('e, 'r, 's) ktree \<Rightarrow> bool" (infix "\<sqsubseteq>" 50) where
 "refined_by P Q = (`itree_pre P \<longrightarrow> itree_pre Q` \<and> {(s, s') \<in> itree_rel Q. itree_pre P s} \<subseteq> itree_rel P)"
 
-lemma assigns_pre: "itree_pre \<langle>\<sigma>\<rangle>\<^sub>a = (True)\<^sub>e"
+lemma assert_pre [dpre]: "itree_pre (assert b) = b"
+  by (auto simp add: itree_pre_def assert_def fun_eq_iff)
+
+lemma assume_pre [dpre]: "itree_pre (assume b) = (True)\<^sub>e"
+  by (auto simp add: itree_pre_def test_def fun_eq_iff)
+     (metis deadlock_def deadlock_trace_to diverge_not_Vis)
+
+lemma assigns_pre [dpre]: "itree_pre \<langle>\<sigma>\<rangle>\<^sub>a = (True)\<^sub>e"
   by (auto simp add: itree_pre_def assigns_def)
 
-lemma Div_pre: "itree_pre Div = (False)\<^sub>e"
+lemma Div_pre [dpre]: "itree_pre Div = (False)\<^sub>e"
   by (auto simp add: itree_pre_def fun_eq_iff)
 
 lemma Div_bottom: "Div \<sqsubseteq> P"
   by (simp add: refined_by_def Div_rel Div_pre)
 
-lemma Stop_pre: "itree_pre Stop = (True)\<^sub>e"
+lemma Stop_pre [dpre]: "itree_pre Stop = (True)\<^sub>e"
   by (auto simp add: itree_pre_def fun_eq_iff deadlock_def)
 
-lemma seq_pre: "itree_pre (P \<Zcomp> Q) = (itree_pre P \<and> wlp P (itree_pre Q))\<^sub>e"
+lemma seq_pre [dpre]: "itree_pre (P \<Zcomp> Q) = (itree_pre P \<and> wlp P (itree_pre Q))\<^sub>e"
   apply (expr_simp, auto elim!: trace_to_bindE simp add: kleisli_comp_def itree_pre_def wlp_itree_def itree_rel_def retvals_def)
   apply (metis bind_diverge trace_to_bind_left)
   apply (meson trace_to_bind)
   apply (metis trace_of_Sils trace_to_Nil trace_to_trans)
   done
 
-lemma input_in_pre:
+lemma input_in_pre [dpre]:
   "wb_prism c \<Longrightarrow> itree_pre (input_in c A P) = (\<forall> v \<in> A. itree_pre (P v))\<^sub>e"
   by (expr_simp add: itree_pre_div_free input_in_where_def div_free_bind div_free_inp_in retvals_inp_in)
 
